rocq/automation/ltac2/UnfoldFix.v
@@ -7,16 +7,24 @@ From impboot Require Import Ltac2Utils ltac2.Constrs ltac2.Stdlib2 ltac2.Message
 (* - Currently it throws No_value, if a non polymorphic reference to a polymorphic function is passed *)
 
 Ltac2 Type exn ::= [
-  UnfoldFixError (message)
+  CannotUnfold (constr)
 ].
 
 Ltac2 reference_to_string (r : reference) : string option :=
   Some (Ident.to_string (List.last (Env.path r))).
 
-Ltac2 unfold_fix_impl (fconstr: constr): unit :=
-  let fref := reference_of_constr fconstr in
-  let unfolded := Std.eval_unfold [(fref, AllOccurrences)] fconstr in
-  match Unsafe.kind unfolded with
+Ltac2 rec apply_to_hyps (c: constr) (hyps: ident list): constr :=
+  match hyps with
+  | [] => c
+  | h :: hs =>
+    let hyp := Control.hyp h in
+    apply_to_hyps open_constr:($c $hyp) hs
+  end.
+
+(* Set Printing All. *)
+
+Ltac2 rec unfold_fix_go (fconstr: constr) (c: constr): unit :=
+  match Unsafe.kind c with
   | Fix structs _i bs cs =>
     let body := Array.get cs 0 in
     let struct := Array.get structs 0 in
@@ -43,26 +51,39 @@ Ltac2 unfold_fix_impl (fconstr: constr): unit :=
     let res := fun () => Std.eval_cbv beta (res ()) in
     let res := fun () => lambda_to_prod (res ()) in
     Control.refine res
+  | Lambda _ _ =>
+    let bs := binders_of_lambda c in
+    let res := Constrs.in_contexts bs (fun () =>
+      let nms := List.map (fun b => Option.get (Binder.name b)) bs in
+      open_constr:(ltac2:(unfold_fix_go (apply_to_hyps fconstr nms) (Std.eval_cbv beta (apply_to_hyps c nms))))
+    ) in
+    let res := fun () => Std.eval_cbv beta (res ()) in
+    let res := fun () => lambda_to_prod (res ()) in
+    Control.refine res
   | _ =>
-    Control.throw (Oopsie (fprintf "Wrong definition passed to unfold_fix_tpe, namely %t" fconstr))
+    Control.throw (CannotUnfold c)
   end.
 
-Ltac2 unfold_fix_gen (fconstr: constr): unit :=
+Ltac2 unfold_fix_impl (fconstr: constr): unit :=
   let fref := reference_of_constr fconstr in
+  let unfolded: constr := Std.eval_unfold [(fref, AllOccurrences)] fconstr in
+  unfold_fix_go fconstr unfolded.
+
+Ltac2 unfold_fix_gen (fconstr: constr): unit :=
+  let _fref := reference_of_constr fconstr in
   let unfolded_fix_template := open_constr:(ltac2:(unfold_fix_impl fconstr)) in
   ltac1:(unfolded_fix_template |- instantiate(1 := unfolded_fix_template)) (Ltac1.of_constr unfolded_fix_template);
   let nms := prod_binder_names (Control.goal ()) in
   Std.intros false (List.map (fun nm => IntroNaming (IntroFresh nm)) nms);
   let struct_name := List.nth nms (Constrs.struct_of_fix fconstr) in
   let struct_hyp := Control.hyp struct_name in
-  (* Std.case true (struct_hyp, NoBindings); *)
-  destruct $struct_hyp eqn:Heqleft at 1;
+  intros;
+  destruct $struct_hyp;
   Control.enter (fun () =>
-    destruct $struct_hyp eqn:Heqright at 1;
     Control.enter (fun () =>
-      rewrite &Heqleft in Heqright; inversion Heqright; subst;
       Control.plus (fun () => (ltac1:(congruence))) (fun _ =>
-        unfold $fref; fold $fconstr;
+        (* TODO: simpl handles more cases here, but it's less predictable *)
+        simpl;
         reflexivity ()
       )
     )
@@ -84,36 +105,3 @@ Ltac2 unfold_fix_proof (fconstr: constr): unit :=
     unfold $fref; fold $fconstr;
     reflexivity ()
   ).
-
-(* Examples *)
-
-(* Fixpoint sum_n (n : nat) : nat :=
-  match n with
-  | 0 => 0
-  | S n1 => (sum_n n1) + n
-  end.
-Lemma sum_n_equation : ltac2:(unfold_fix_type 'sum_n). *)
-
-Fixpoint sum_n1 (n : nat) : nat :=
-  match n with
-  | 0 => 0
-  | S n1 => (sum_n1 n1) + (n1 + 1)
-  end.
-Lemma sum_n1_equation : ltac2:(unfold_fix_type 'sum_n1).
-Proof. unfold_fix_proof 'sum_n1. Qed.
-
-Fixpoint is_even (n: nat): bool :=
-  match n with
-  | 0 => true
-  | S n1 => is_odd n1
-  end
-with is_odd (n: nat): bool :=
-  match n with
-  | 0 => false
-  | S n1 => is_even n1  
-  end.
-Print is_even.
-(* TODO: fix me *)
-Lemma is_even_equation: ltac2:(unfold_fix_type 'is_even).
-Proof. unfold_fix_proof 'is_even. Qed.
-About is_even_equation.
