rocq/imp2asm/ImpToASMCodegen.v
@@ -555,7 +555,7 @@ Fixpoint c_fndefs (ds: list func) (l: nat) (fs: f_lookup): (asm_appl * list (nam
     let/d fname := func_nm d in
     let/d '(c1, l1) := c_fundef d (l + 1) fs in
     let/d '(c2, fs', l2) := c_fndefs ds' (l1 + 1) fs in
-    let/d comment := List [Comment (N2asciid fname)] in
+    let/d comment := List [Comment (N2ascii fname)] in
     (comment +++ c1 +++ List [Ret] +++ c2, (fname, (l + 1)) :: fs', l2)
   end.
 Theorem c_fndefs_equation: ltac2:(unfold_fix_type '@c_fndefs).
